src/case_study/stack_transform.v
@@ -46,6 +46,124 @@ Lemma push_stack_length s :
   length (push_stack s) = S (length s).
 Proof. induction s; simpl; auto. Qed.
 
+Lemma list_to_gmap_stack_fix_lookup_is_Some s n m :
+  is_Some (list_to_gmap_stack_fix s n !! m) ->
+  m < length s + n.
+Proof.
+  revert n m; induction s;intros n m.
+  - simpl. intros [? ?];done.
+  - simpl. intros Hx.
+    destruct (decide (n = m));subst.
+    + simplify_map_eq. lia.
+    + rewrite lookup_insert_ne// in Hx.
+      apply IHs in Hx. lia.
+Qed.
+Lemma list_to_gmap_stack_fix_lookup_Some s n m v :
+  list_to_gmap_stack_fix s n !! m = Some v ->
+  m < length s + n.
+Proof.
+  intros Hsome.
+  apply list_to_gmap_stack_fix_lookup_is_Some.
+  eauto.
+Qed.
+
+Lemma list_to_gmap_stack_lookup_is_Some s m l :
+  is_Some (list_to_gmap_stack s !! (m, l)) ->
+  m < length s.
+Proof.
+  intros [x Hx].
+  unfold list_to_gmap_stack in Hx.
+  rewrite lookup_gmap_uncurry in Hx.
+  destruct (list_to_gmap_stack_fix s 0 !! m) eqn:Hsome;try done.
+  apply list_to_gmap_stack_fix_lookup_Some in Hsome. lia.
+Qed.
+Lemma list_to_gmap_stack_lookup_Some s m l v :
+  list_to_gmap_stack s !! (m, l) = Some v ->
+  m < length s.
+Proof.
+  intros Hsome.
+  eapply list_to_gmap_stack_lookup_is_Some;eauto.
+Qed.
+
+Lemma list_to_gmap_stack_fix_snoc_mid s x n :
+  (list_to_gmap_stack_fix (s ++ [x]) n) = <[n + (length s) := x]> (list_to_gmap_stack_fix s n).
+Proof.
+  revert n. induction s;intros n.
+  - rewrite app_nil_l /= PeanoNat.Nat.add_0_r. auto.
+  - simpl.  rewrite IHs. rewrite insert_commute;[|lia].
+    assert (S n + length s = n + S (length s)) as ->;[lia|].
+    auto.
+Qed.
+
+Lemma list_to_gmap_stack_fix_snoc s x :
+  (list_to_gmap_stack_fix (s ++ [x]) 0) = <[(length s) := x]> (list_to_gmap_stack_fix s 0).
+Proof.
+  assert (length s = 0 + length s) as ->;[lia|].
+  apply list_to_gmap_stack_fix_snoc_mid.
+Qed.
+
+Lemma list_to_gmap_lookup_snoc s x m l :
+  m < length s ->
+  list_to_gmap_stack (s ++ [x]) !! (m, l) = list_to_gmap_stack s !! (m, l).
+Proof.
+  revert m. induction s using rev_ind;intros m Hle.
+  - simpl in *. destruct m;lia.
+  - destruct (decide (m = length s)).
+    + subst. rewrite /list_to_gmap_stack /= !lookup_gmap_uncurry.
+      rewrite list_to_gmap_stack_fix_snoc. rewrite app_length /=.
+      rewrite lookup_insert_ne//. lia.
+    + rewrite app_length /= in Hle. assert (m < length s) as Hlt;[lia|].
+      apply IHs in Hlt.
+      rewrite /list_to_gmap_stack /= !lookup_gmap_uncurry.
+      rewrite list_to_gmap_stack_fix_snoc.
+      rewrite lookup_insert_ne;[|rewrite app_length;lia].
+      rewrite /list_to_gmap_stack /= !lookup_gmap_uncurry in Hlt.
+      auto.
+Qed.
+
+Lemma list_to_gmap_stack_fix_lookup s n m l :
+  n <= m ->
+  list_to_gmap_stack_fix s n !! m ≫= lookup l = s !! (m - n) ≫= (λ σ : gmap loc val, σ !! l).
+Proof.
+  revert n. induction s;intros n Hle.
+  - simpl. auto.
+  - simpl. destruct (decide (n = m)).
+    + subst. rewrite lookup_insert Nat.sub_diag /= //.
+    + assert (S n <= m);[lia|].
+      rewrite lookup_insert_ne // IHs //.
+      assert (m - n = S (m - S n)) as ->;[lia|].
+      simpl. auto.
+Qed.    
+
+Lemma list_to_gmap_stack_lookup (s : list (gmap loc val)) (m : nat) (l : loc) :
+  (list_to_gmap_stack s) !! (m, l) = s !! m ≫= λ σ, σ !! l.
+Proof.
+  rewrite /list_to_gmap_stack.
+  rewrite lookup_gmap_uncurry.
+  rewrite list_to_gmap_stack_fix_lookup;[|lia].
+  rewrite Nat.sub_0_r. auto.
+Qed.
+
+Lemma list_to_gmap_stack_insert s s0 l v n :
+  s !! n = Some s0 ->
+  <[(n, l) := v]> (list_to_gmap_stack s) = list_to_gmap_stack (<[n :=<[l:=v]>s0]> s).
+Proof.
+  intros Hl. apply map_eq.
+  intros [n' l'].
+  rewrite list_to_gmap_stack_lookup.
+  apply lookup_lt_Some in Hl as Hlt.
+  destruct (decide ((n',l') = (n, l))).
+  - simplify_eq.
+    rewrite lookup_insert list_lookup_insert// /=.
+    rewrite lookup_insert //.
+  - rewrite lookup_insert_ne//.
+    rewrite list_to_gmap_stack_lookup.
+    destruct (decide (n' = n)).
+    + subst. rewrite list_lookup_insert// Hl /=.
+      rewrite lookup_insert_ne//. intros Hcontr;subst. done.
+    + rewrite list_lookup_insert_ne//.
+Qed.
+
 Section pop_func.
 
   Definition stackM := gmap_view.gmap_viewUR (nat * loc) (leibnizO val).
@@ -130,23 +248,6 @@ Section pop_func.
     rewrite /stack_cut /stack_cond. rewrite map_filter_id//.
     intros [m l] x Hx. apply elem_of_dom_2 in Hx. apply Hgt in Hx. auto.
   Qed.
-  
-  Lemma list_to_gmap_stack_fix_snoc_mid s x n :
-    (list_to_gmap_stack_fix (s ++ [x]) n) = <[n + (length s) := x]> (list_to_gmap_stack_fix s n).
-  Proof.
-    revert n. induction s;intros n.
-    - rewrite app_nil_l /= PeanoNat.Nat.add_0_r. auto.
-    - simpl.  rewrite IHs. rewrite insert_commute;[|lia].
-      assert (S n + length s = n + S (length s)) as ->;[lia|].
-      auto.
-  Qed.
-  
-  Lemma list_to_gmap_stack_fix_snoc s x :
-    (list_to_gmap_stack_fix (s ++ [x]) 0) = <[(length s) := x]> (list_to_gmap_stack_fix s 0).
-  Proof.
-    assert (length s = 0 + length s) as ->;[lia|].
-    apply list_to_gmap_stack_fix_snoc_mid.
-  Qed.
 
   Lemma stack_cut_snoc s n m x l :
     n <= m ->
@@ -167,98 +268,81 @@ Section pop_func.
     rewrite decide_True//.
   Qed.
 
-  Lemma list_to_gmap_stack_fix_lookup_is_Some s n m :
-    is_Some (list_to_gmap_stack_fix s n !! m) ->
-    m < length s + n.
+  Lemma popN_stack_lookup_Some s1 i n g :
+    popN_stack s1 i !! n = Some g ->
+    s1 !! n = Some g.
   Proof.
-    revert n m; induction s;intros n m.
-    - simpl. intros [? ?];done.
-    - simpl. intros Hx.
-      destruct (decide (n = m));subst.
-      + simplify_map_eq. lia.
-      + rewrite lookup_insert_ne// in Hx.
-        apply IHs in Hx. lia.
-  Qed.
-  Lemma list_to_gmap_stack_fix_lookup_Some s n m v :
-    list_to_gmap_stack_fix s n !! m = Some v ->
-    m < length s + n.
-  Proof.
-    intros Hsome.
-    apply list_to_gmap_stack_fix_lookup_is_Some.
-    eauto.
-  Qed.
-      
-  Lemma list_to_gmap_stack_lookup_is_Some s m l :
-    is_Some (list_to_gmap_stack s !! (m, l)) ->
-    m < length s.
-  Proof.
-    intros [x Hx].
-    unfold list_to_gmap_stack in Hx.
-    rewrite lookup_gmap_uncurry in Hx.
-    destruct (list_to_gmap_stack_fix s 0 !! m) eqn:Hsome;try done.
-    apply list_to_gmap_stack_fix_lookup_Some in Hsome. lia.
-  Qed.
-  Lemma list_to_gmap_stack_lookup_Some s m l v :
-    list_to_gmap_stack s !! (m, l) = Some v ->
-    m < length s.
-  Proof.
-    intros Hsome.
-    eapply list_to_gmap_stack_lookup_is_Some;eauto.
+    revert s1 n g. induction i;intros s1 n g.
+    - simpl. auto.
+    - simpl. intros Hs.
+      unfold pop_stack in Hs.
+      destruct s1 using rev_ind;auto.
+      clear IHs1. rewrite reverse_snoc reverse_involutive in Hs.
+      apply IHi in Hs. rewrite lookup_app_l//.
+      apply lookup_lt_Some in Hs =>//.
   Qed.
 
-  Lemma list_to_gmap_lookup_snoc s x m l :
-    m < length s ->
-    list_to_gmap_stack (s ++ [x]) !! (m, l) = list_to_gmap_stack s !! (m, l).
+  Lemma popN_stack_length s i :
+    length (popN_stack s i) = length s - i.
   Proof.
-    revert m. induction s using rev_ind;intros m Hle.
-    - simpl in *. destruct m;lia.
-    - destruct (decide (m = length s)).
-      + subst. rewrite /list_to_gmap_stack /= !lookup_gmap_uncurry.
-        rewrite list_to_gmap_stack_fix_snoc. rewrite app_length /=.
-        rewrite lookup_insert_ne//. lia.
-      + rewrite app_length /= in Hle. assert (m < length s) as Hlt;[lia|].
-        apply IHs in Hlt.
-        rewrite /list_to_gmap_stack /= !lookup_gmap_uncurry.
-        rewrite list_to_gmap_stack_fix_snoc.
-        rewrite lookup_insert_ne;[|rewrite app_length;lia].
-        rewrite /list_to_gmap_stack /= !lookup_gmap_uncurry in Hlt.
-        auto.
+    revert s;induction i;intros s.
+    - rewrite /=. lia.
+    - simpl.  specialize (IHi (pop_stack s)).
+      rewrite IHi. rewrite /pop_stack.
+      destruct s using rev_ind;simpl;[lia|].
+      rewrite reverse_snoc reverse_involutive.
+      rewrite app_length /=. lia.
+  Qed.      
+
+  Lemma popN_stack_lookup_lt s1 i n g :
+    popN_stack s1 i !! n = Some g ->
+    n < length s1 - i.
+  Proof.
+    intros Hs. apply lookup_lt_Some in Hs.
+    rewrite popN_stack_length in Hs. auto.
   Qed.
 
-  (* Lemma list_to_gmap_lookup_stack_cut n s m l : *)
-  (*   m < n -> *)
-  (*   (list_to_gmap_stack (stack_cut n s)) !! (m, l) = (list_to_gmap_stack s) !! (m, l). *)
-  (* Proof. *)
-  (*   intros Hlt. *)
-  (*   destruct (list_to_gmap_stack s !! (m, l)) eqn:Hsome. *)
-  (*   - apply list_to_gmap_stack_lookup_Some in Hsome as Hlt'. *)
-  (*     rewrite /list_to_gmap_stack lookup_gmap_uncurry. *)
-  (*     rewrite /list_to_gmap_stack lookup_gmap_uncurry in Hsome. *)
-  (*     destruct (list_to_gmap_stack_fix s 0 !! m) eqn:Hsome';[|done]. *)
-  (*     simpl in Hsome.  *)
+  Lemma popN_stack_lookup_None s1 i n :
+    popN_stack s1 i !! n = None ->
+    s1 !! n = None \/ n >= length s1 - i.
+  Proof.
+    revert s1 n. induction i;intros s1 n.
+    - simpl. auto.
+    - simpl. intros Hs.
+      unfold pop_stack in Hs.
+      destruct s1 using rev_ind;auto.
+      clear IHs1. rewrite reverse_snoc reverse_involutive in Hs.
+      apply IHi in Hs as [Hnone | Hge].
+      + destruct (decide (n = length s1)).
+        * subst. right. rewrite app_length /=.
+          lia.
+        * apply lookup_ge_None_1 in Hnone as Hge.
+          assert (length s1 < n);[lia|].
+          rewrite lookup_ge_None_2;auto.
+          rewrite app_length /=. lia.
+      + right. rewrite app_length /=. lia.
+  Qed.
 
-      
-  (* Admitted. *)
-
-  (* Lemma stack_cut_list_to_gmap_stack (s : stack) (n : nat) : *)
-  (*   stack_cut_rel n (list_to_gmap_stack s) (list_to_gmap_stack (stack_cut n s)). *)
-  (* Proof. *)
-  (*   revert n; induction s using rev_ind;intros n. *)
-  (*   - unfold list_to_gmap_stack. *)
-  (*     constructor;auto. *)
-  (*   - (* unfold list_to_gmap_stack. *) *)
-  (*     (* rewrite list_to_gmap_stack_fix_snoc. *) *)
-  (*     (* rewrite stack_cut_snoc. *) *)
-  (*     constructor. *)
-  (*     + intros m l v Hsome Hlt. *)
-  (*       apply list_to_gmap_stack_lookup_Some in Hsome as Hlt'. *)
-  (*       (* unfold list_to_gmap_stack. *) *)
-  (*       rewrite app_length /= in Hlt'. *)
-  (*       destruct (decide (n <= length s)). *)
-  (*       * rewrite stack_cut_snoc//. *)
-  (*         assert (m < length s);[lia|]. *)
-  (*         rewrite list_to_gmap_lookup_snoc// in Hsome. *)
-  (* Admitted. *)
+  Lemma stack_location_cut_popN_stack s1 i :
+    map_imap (stack_location_cut (length s1 - i)) (list_to_gmap_stack s1) = list_to_gmap_stack (popN_stack s1 i).
+  Proof.
+    apply map_eq.
+    intros [n l]. rewrite list_to_gmap_stack_lookup.
+    rewrite map_lookup_imap list_to_gmap_stack_lookup.
+    destruct (popN_stack s1 i !! n) eqn:Hsome1.
+    - apply popN_stack_lookup_Some in Hsome1 as Hsome2.
+      rewrite Hsome2 Hsome1 /= /stack_location_cut /=.
+      destruct (g !! l) =>// /=.
+      rewrite bool_decide_eq_true_2 //.
+      rewrite /stack_cond /=.
+      apply popN_stack_lookup_lt in Hsome1. auto.
+    - apply popN_stack_lookup_None in Hsome1 as Hnone.
+      destruct Hnone as [Hnone|Hge];[rewrite Hnone Hsome1 /= //|].
+      rewrite Hsome1 /=. destruct (s1 !! n) eqn:Hnone;auto.
+      simpl. destruct (g !! l) eqn:Hl;auto.
+      simpl. rewrite /stack_location_cut bool_decide_eq_false_2//.
+      rewrite /stack_cond /=. lia.
+  Qed.
   
   
 End pop_func.
